Arbitrary intermediate point in verifying Depl statement compiler

platform/Depl/Compile.v
@@ -1,6 +1,6 @@
 (** Compiling the deeply embedded programming language *)
 
-Require Import AutoSep Wrap.
+Require Import AutoSep Wrap Malloc.
 
 Require Import Depl.Logic Depl.Cancel Depl.AlgebraicDatatypes Depl.Statements.
 
@@ -49,3 +49,115 @@ Proof.
   rewrite rupd_eq in Hsome; subst.
   eauto.
 Qed.
+
+
+(** * Lowering statements *)
+
+Fixpoint stmtC (s : stmt) : chunk :=
+  match s with
+    | Assign x e => x <- exprC e
+    | Seq s1 s2 => stmtC s1;; stmtC s2
+    | Ret e => Return (exprC e)
+  end%SP.
+
+(** Version of [Logic.predD] specialized to predicates with no free higher-order variables *)
+Definition predD (p : pred) (fE : fo_env) : HProp :=
+  predD p (fun _ _ => Emp)%Sep fE.
+
+(** Helper to copy formal parameter values from a [vals] to a [fo_env] *)
+Fixpoint formals (V : vals) (xs : list pr_var) (fE : fo_env) : fo_env :=
+  match xs with
+    | nil => fE
+    | x :: xs => fo_set (formals V xs fE) x (Dyn (sel V x))
+  end.
+
+(** Generic precondition of a statement, translated to base Bedrock from Depl-speak *)
+Definition precond (vs : vars) (pre post : pred) :=
+  (* First, quantify over a context assigning values to specification variables. *)
+  Al fE,
+    (* Naturally, we rely on the malloc() data structures being around. *)
+    PRE[V] mallocHeap 0
+      (* We also need the Depl precondition, of course. *)
+      * predD pre fE
+      (* Finally, the symbolic variable valuation should be accurate. *)
+      * [| vars_ok fE V vs |]
+    POST[R] mallocHeap 0
+      (* The postcondition holds, in an [fo_env] that lets it mention the return value. *)
+      * predD post (fo_set fE "result" (Dyn R)).
+
+(** Generic postcondition of a statement *)
+Definition postcond (vs : vars) (pre post : pred) (s : stmt) :=
+  match stmtD vs s with
+    | Error =>
+      (* It's going to crash.  No guarantees! *)
+      fun _ _ _ _ => st ~> [| True |]
+    | Returned _ =>
+      (* We returned already.  Unreachable! *)
+      PREonly[_] [| False |]
+    | Success vs' =>
+      (* Still executing. *)
+      precond vs' pre post
+  end.
+
+(** * Key lemmas to pass to Wrap *)
+
+Lemma Stmt_post : forall xs vs pre post im mn (H : importsGlobal im) ns res pre0 specs,
+  (forall specs0 st0,
+    interp specs0 (pre0 st0)
+    -> interp specs0 (precond vs pre post true (fun x => x) ns res st0))
+  -> incl xs ns
+  -> (forall x, In x xs -> vs x <> None)
+  -> forall s st,
+    stmtV xs s
+    -> interp specs (Structured.Postcondition (toCmd (stmtC s) mn H ns res pre0) st)
+    -> interp specs (postcond vs pre post s true (fun x => x) ns res st).
+Proof.
+  induction s; post; intuition; unfold postcond.
+
+  match goal with
+    | [ H : interp _ _, H' : forall specs0 : codeSpec _ _, _ |- _ ] =>
+      apply H' in H; clear H'; post
+  end.
+
+  match goal with
+    | [ |- context[match ?E with None => _ | _ => _ end] ] =>
+      match E with
+        | context[match _ with None => _ | _ => _ end] => fail 1
+        | _ => case_eq E; post
+      end
+  end.
+  specialize (H2 _ H4).
+  match goal with
+    | [ |- context[match ?E with None => _ | _ => _ end] ] =>
+      match E with
+        | context[match _ with None => _ | _ => _ end] => fail 1
+        | _ => case_eq E; post
+      end
+  end.
+  
+
+  case_eq (exprD vs e); post.
+  
+  
+
+
+
+(** Main statement compiler/combinator/macro *)
+Definition Stmt
+  (xs : list pr_var)
+  (* Program variables available to mention *)
+  (vs : vars)
+  (* Symbolic valuation to those variables *)
+  (pre post : pred)
+  (* The Depl-level separation-logic specification for this statement *)
+  (s : stmt)
+  (* The statement to compile *)
+  : chunk.
+  apply (WrapC (stmtC s)
+    (precond vs pre post)
+    (postcond vs pre post s)
+
+    (* VERIFICATION CONDITION *)
+    (fun _ xs' _ =>
+      incl xs xs'
+      :: nil)).
